## Setup
- Let $\mathscr{C}$ be a category. A set of models simply means a subset $\mathcal{M}\subset\operatorname{Ob}(\mathscr{C})$. Fix a set map $I\to\mathcal{M}$.
- We say that a functor $T:\mathscr{C}\to\mathsf{Ab}$ (or $R\text{-}\mathsf{Mod}$) is
	- Free on $\mathcal{M}$ with model basis $\{x_i\in T(M_i):i\in I,\,M_i\in\mathcal{M}\}$, if for all $C\in\operatorname{Ob}(\mathscr{C})$, the set $\{T(f)(x_i):i\in I,\, f\in\operatorname{Hom}(M_i,C)\}$ is a basis for $T(C)$.
- Lemma. If $T$ is free on $\mathcal{M}$, then it is a projective in the category $\mathsf{Ab}^{\mathscr{C}}=\mathsf{Fct}(\mathscr{C},\mathsf{Ab})$.
	- Proof. First, observe that $T=\bigoplus_{i\in I}T_i$ because colimits are pointwise in the functor category, where $T_i$ is a functor that's free on a single model $\{M_i\}$ with basis $\{x_i\}$. By how projectives work, we may assume $|I|=1$ and $\mathcal{M}=\{M\}$.
	- Consider the adjunction pair $\operatorname{Free}:\mathsf{Set}\rightleftarrows\mathsf{Ab}:\operatorname{U}$. Because the isomorphism $\varphi\leftrightarrow\psi$ is given by "absolute"/"natural" equations (viz. $\psi=\operatorname{U}\varphi\circ\eta$), this easily lifts an adjunction
	- $$\operatorname{Free}_*:\mathsf{Set}^{\mathscr{C}}\rightleftarrows\mathsf{Ab}^{\mathscr{C}}:\operatorname{U}_*$$
	- By the Yoneda lemma, $x\in UT(M)$ gives a natural transformation $\operatorname{Hom}(M,-)=:k_M\to U_*T$, such that the corresponding $\operatorname{Free}_*k_M\to T$ is an isomorphism by assumption. Hence
	- $$\operatorname{Hom}(T,Z)=\operatorname{Hom}(k_M,U_*Z)\simeq Z(M),\quad \phi\mapsto\phi(M)(x),$$
	- Which implies that $T$ is projective since $Z\mapsto Z(M)$ is exact. QED
- Remark. For the acyclic models theorem, as projectivity is not quite enough, we use the above Yoneda isomorphism. So this lemma is just for the concept.
- Now consider a functor $T_\bullet:\mathscr{C}\to\mathsf{Ch}_{\geq0}(\mathsf{Ab})$. We say it is
	- Free on $\mathcal{M}$, if $T_n$ is free on $\mathcal{M}$ for all $n\geq 0$.
	- Acyclic on $\mathcal{M}$, if $T(M)$ is acyclic for all $M\in\mathcal{M}$.
- Denote its $n$-th homology as $H_n(T_\bullet)$.
- ## The theorem
- Theorem (Acyclic models). If $T_\bullet$ is free on $\mathcal{M}$ and $S_\bullet$ is acyclic on $\mathcal{M}$, then for any natural transformation $\theta:H_0(T_\bullet)\to H_0(S_\bullet)$, there exists a natural chain map $\Theta:T_\bullet\to S_\bullet$ inducing it. Moreover, $\Theta$ is unique up to natural chain homotopy.
  background-color:: yellow
	- Proof. This is very basic.
	- Since $S_\bullet\to H_0(S_\bullet)\to 0$ is exact on $\mathcal{M}$, the existence of $\Theta$ reduces to the following: If $X\xrightarrow{\partial} Y\xrightarrow{\partial} Z$ is exact on $\mathcal{M}$, $T$ is free on $\mathcal{M}$ and $f:T\to Y$ satisfies $\partial f=0$, then there exists $g:T\to X$ such that $f=\partial g$.
	- We then reduce to case when $T=\operatorname{Free}_*k_M$, then apply $\operatorname{Hom}(T,-)=\operatorname{ev}_M(-)$. See above lemma. Existence is established.
	- Now, suppose $\Theta$ and $\Theta'$ both induces $\theta$ at $n=0$, we need to inductively build $h:T_\bullet\to S_\bullet[1]$ such that $\partial_{n+1}h_n+h_{n-1}\partial_n=\Theta_n-\Theta'_n=:\varphi_n$. Put $h_n=0$ for $n<0$, and suppose we have constructed up to $h_{n-1}$. Then
	- $$\partial_n(\varphi_n-h_{n-1}\partial_n)=(\varphi_{n-1}-\partial_nh_{n-1})\partial_n=h_{n-2}\partial_{n-1}\partial_n=0.$$
	- Use above logic again, we find $h_n$ such that $\partial h_n=\varphi_n-h_{n-1}\partial_n$. QED
- Corollary. If both $T_\bullet,S_\bullet$ are free and acyclic on $\mathcal{M}$, and if $\theta:H_0(T_\bullet)\xrightarrow{\sim}H_0(S_\bullet)$, then any natural chain map $\Theta$ inducing $\theta$ is a natural homotopy equivalence. In particular, such $\Theta$ exists, so $T_\bullet$ and $S_\bullet$ have isomorphic homology groups.
- ## Applications
- ### Homotopy invariance of singular homology
- Consider the two embeddings $\iota_0,\iota_1:X\to X\times I$. Given two continuous maps $f,g:X\to Y$, a homotopy $f\simeq g$ is $H:X\times I\to Y$ satisfying $H\iota_0=f$, $H\iota_1=g$.
- We want to show that $f_*=g_*$ at *homology* level. It suffices to prove $f_*$ and $g_*$ are homotopic at *chain* level.
- Proposition. The induced chain maps $(\iota_0)_*$ and $(\iota_1)_*$ are homotopic.
	- Proof. $\iota_0$ is a natural transformation, and so is $(\iota_0)_*=S_\bullet\iota_0:S_\bullet\to T_\bullet$, where $T_\bullet(-):=S_\bullet(-\times I)$. On $\mathscr{C}=\mathsf{Top}$, we choose $\mathcal{M}=\{\Delta^p\}_{p\geq0}$. Then each $S_n$ is free on the basis $\{\mathrm{id}_{\Delta^n}\}$.
	- It is clear that $H_0(\iota_0)=H_0(\iota_1)$.
	- To apply the uniqueness of the theorem, it remains to check that $T_\bullet$ is acyclic on $\mathcal{M}$. This is done by the following lemma. QED
- Lemma. The reduced homology of any convex subset $D$ of an Euclidean space is $0$.
  background-color:: yellow
	- Proof. Pick an arbitrary "apex" $a\in D$. Define the cone operator $K:S_\bullet(D)\to S_\bullet(D)[1]$ which, on an $n$-simplex $\sigma$, is given by
	- $$(K\sigma)(t_0,\cdots,t_{n+1})=t_0a+(1-t_0)\sigma\left(\frac{t_1}{1-t_0},\cdots,\frac{t_{n+1}}{1-t_0}\right).$$
	- Suppose $n\geq1$ and we compute the $i$-th faces of $K\sigma$, $0\leq i\leq n+1$. If $i=0$, we get $(K\sigma)d_i=\sigma$. If $i>1$, we clearly have $(K\sigma)d_i=K(\sigma d_{i-1})$. Hence
	- $$\partial K+K\partial=\mathrm{id}.$$
	- Finally, if $n=1$, $Kx$ is a line from $x\in D$ to $a$, so $\partial Kx=x-a$. Hence
	- $$\partial K+K\epsilon=\mathrm{id},$$
	- where $\epsilon:S_0(D)\to\mathbb{Z}$ is the augmentation map. QED
- ### Simplicial homology = Singular homology